src/tc/normalize.fsi
@@ -22,7 +22,6 @@ open Microsoft.FStar.Tc
 open Microsoft.FStar.Absyn.Syntax
  
 type step = 
-  | Alpha           
   | Delta        (* don't expand abbreviations if they aren't blocking reduction *)
   | DeltaHard    (* expand all abbreviations *)
   | Beta
